修改了findref部分注释，尝试证明

HashTable/hashtbl.c
@@ -119,25 +119,29 @@ unsigned int *hashtbl_findref(struct hashtbl *h, char *key)
   ind = hash_string(key) % 211;
   i = &h->bucks[ind];
   /*@ Inv Assert
-      exists l l0 l_prev l_res k0 k_list lh b0 buck,
+      exists l l0 l_prev l_res lh b0 buck,
       contain_all_addrs(m, l) && 
       repr_all_heads(lh, b0) && 
       contain_all_correct_addrs(m, b0) && 
-      not_key(k, l_prev) &&
       0 <= ind && ind < 211 &&
       b0(ind) == Some(pair(&(h->bucks[ind]),l0)) &&
+      not_key(key, l_prev) &&
       l0 == app(l_prev, l_res) &&
-      m(k_list) == Some(&(*i)->val) &&
+      store(&(h->bucks[ind]),buck) &&
+      sllseg(&(h->bucks[ind]), *i, l_prev) *
+      ((*i == (void *) 0 && l_res == nil) || 
+      (*i != (void *) 0 && 
+        exists p_current l_resres key_addr k_list_current,
+          *i == p_current &&
+          l_res == cons(p_current, l_resres) &&
+          store_ptr(&(p_current->key), key_addr) *
+          store_string(key_addr, k_list_current) *
+          sll(p_current, l_res))) &&
       store_map(store_sll, b0)*
       dll(h->top, (void*) 0, l) * 
       IntArray::full(h->bucks, 211, lh)*
-      sllseg(&(h->bucks[ind]), (*i), l_prev) *
-      sll((*i), l_res) *
-      store_ptr(&(*i)->key, k0)*
-      store_string(k0, k_list) *
       store_string(key, k) *
-      store_map(store_name, m) *
-      store(&(h->bucks[ind]),buck)
+      store_map(store_name, m)
   */
   //Inv的最后三句是为了string_equal,*i = b->next和b->next = h->bucks[ind]不会报错
   for (; *i != (void *) 0; i = &(*i)->next){
@@ -154,199 +158,199 @@ unsigned int *hashtbl_findref(struct hashtbl *h, char *key)
 }
 
 
-unsigned int hashtbl_remove(struct hashtbl *h, char *key, int *removed)
-/*@
-  With m1 m2 k
-  Require map_composable(m1, m2) &&
-          store_hash_skeleton(h, m1) *
-          store_map(store_uint, m2) *
-          store_string(key, k) *
-          has_int_permission(removed)
-  Ensure store_hash_skeleton(h, KP::remove_map(m1, k)) *
-         store_string(key, k) *
-         ((exists p v key0,
-             m1(k) == Some(&(p -> val)) &&
-             m2(&(p -> val)) == Some(v) && __return == v &&
-             store_int(removed, 1) *
-             store_map(store_uint, PV::remove_map(m2, p)) *
-             store_ptr(&(p -> key), key0) * store_string(key0, k) *
-             has_ptr_permission(&(p -> up)) *
-             has_ptr_permission(&(p -> down)) *
-             has_ptr_permission(&(p -> next)) *
-             store_uint(&(p -> val), v)) ||
-          (m1(k) == None && __return == 0 &&
-           store_int(removed, 0) * store_map(store_uint, m2)))
-*/
-{
-  unsigned int ind;
-  struct blist **it;
-  /*@ store_hash_skeleton(h, m1)
-      which implies
-        exists l lh b, 
-        contain_all_addrs(m1, l) && 
-        repr_all_heads(lh, b) && 
-        contain_all_correct_addrs(m1, b) && 
-        dll(h->top, (void*) 0, l) * 
-        IntArray::full(h->bucks, 211, lh) * 
-        store_map(store_sll, b)*
-        store_map(store_name, m1)
-  */
-  ind = hash_string(key) % 211;
-  /*@ Inv Assert
-      exists l l0 lh b l_prev l_res k_list k0 buck dl_up dl_down val,
-      map_composable(m1, m2) &&
-      not_key(key, l_prev) &&
-      0 <= ind && ind < 211 &&
-      contain_all_addrs(m1, l) && 
-      repr_all_heads(lh, b) && 
-      contain_all_correct_addrs(m1, b) && 
-      b(ind) == Some(pair(&(h->bucks[ind]),l0)) &&
-      l0 == app(l_prev, l_res) &&
-      l == app(dl_up, dl_down) &&
-      m1(k_list) == Some(&(*it)->val) &&
-      sllseg(buck, (*it), l_prev) *
-      sll((*it), l_res) *
-      store(&h->bucks[ind], buck) *
-      dllseg(h->top, (*it), (void*) 0, (*it)->up, dl_up) *
-      dll((*it), (*it)->up, dl_down) *
-      store_ptr((*it)->up->down, (*it)) *
-      store_ptr((*it)->down->up, (*it)) *
-      store_uint(&(*it)->val, val) *
-      store_ptr(&(*it)->key, k0) *
-      store_string(k0, k_list) *
-      has_int_permission(removed) *
-      store_map(store_name, m1) *
-      store_map(store_uint, m2) *
-      store_string(key, k)
-  */
-  for (it = &h->bucks[ind]; *it != (void *) 0; it = &(*it)->next) {
-    struct blist *b = *it;
-    if (string_equal(key, b->key)) {
-      if (h->top == b)
-        h->top = b->down;
-      if (b->up != (void *) 0)
-        b->up->down = b->down;
-      if (b->down != (void *) 0)
-        b->down->up = b->up;
+// unsigned int hashtbl_remove(struct hashtbl *h, char *key, int *removed)
+// /*@
+//   With m1 m2 k
+//   Require map_composable(m1, m2) &&
+//           store_hash_skeleton(h, m1) *
+//           store_map(store_uint, m2) *
+//           store_string(key, k) *
+//           has_int_permission(removed)
+//   Ensure store_hash_skeleton(h, KP::remove_map(m1, k)) *
+//          store_string(key, k) *
+//          ((exists p v key0,
+//              m1(k) == Some(&(p -> val)) &&
+//              m2(&(p -> val)) == Some(v) && __return == v &&
+//              store_int(removed, 1) *
+//              store_map(store_uint, PV::remove_map(m2, p)) *
+//              store_ptr(&(p -> key), key0) * store_string(key0, k) *
+//              has_ptr_permission(&(p -> up)) *
+//              has_ptr_permission(&(p -> down)) *
+//              has_ptr_permission(&(p -> next)) *
+//              store_uint(&(p -> val), v)) ||
+//           (m1(k) == None && __return == 0 &&
+//            store_int(removed, 0) * store_map(store_uint, m2)))
+// */
+// {
+//   unsigned int ind;
+//   struct blist **it;
+//   /*@ store_hash_skeleton(h, m1)
+//       which implies
+//         exists l lh b, 
+//         contain_all_addrs(m1, l) && 
+//         repr_all_heads(lh, b) && 
+//         contain_all_correct_addrs(m1, b) && 
+//         dll(h->top, (void*) 0, l) * 
+//         IntArray::full(h->bucks, 211, lh) * 
+//         store_map(store_sll, b)*
+//         store_map(store_name, m1)
+//   */
+//   ind = hash_string(key) % 211;
+//   /*@ Inv Assert
+//       exists l l0 lh b l_prev l_res k_list k0 buck dl_up dl_down val,
+//       map_composable(m1, m2) &&
+//       not_key(key, l_prev) &&
+//       0 <= ind && ind < 211 &&
+//       contain_all_addrs(m1, l) && 
+//       repr_all_heads(lh, b) && 
+//       contain_all_correct_addrs(m1, b) && 
+//       b(ind) == Some(pair(&(h->bucks[ind]),l0)) &&
+//       l0 == app(l_prev, l_res) &&
+//       l == app(dl_up, dl_down) &&
+//       m1(k_list) == Some(&(*it)->val) &&
+//       sllseg(buck, (*it), l_prev) *
+//       sll((*it), l_res) *
+//       store(&h->bucks[ind], buck) *
+//       dllseg(h->top, (*it), (void*) 0, (*it)->up, dl_up) *
+//       dll((*it), (*it)->up, dl_down) *
+//       store_ptr((*it)->up->down, (*it)) *
+//       store_ptr((*it)->down->up, (*it)) *
+//       store_uint(&(*it)->val, val) *
+//       store_ptr(&(*it)->key, k0) *
+//       store_string(k0, k_list) *
+//       has_int_permission(removed) *
+//       store_map(store_name, m1) *
+//       store_map(store_uint, m2) *
+//       store_string(key, k)
+//   */
+//   for (it = &h->bucks[ind]; *it != (void *) 0; it = &(*it)->next) {
+//     struct blist *b = *it;
+//     if (string_equal(key, b->key)) {
+//       if (h->top == b)
+//         h->top = b->down;
+//       if (b->up != (void *) 0)
+//         b->up->down = b->down;
+//       if (b->down != (void *) 0)
+//         b->down->up = b->up;
 
-      *it = b->next;
-      unsigned int res = b->val;
-      free_string(b->key);
-      free_blist(b);
-      *removed = 1;
-      return res;
-    }
-  }
-  *removed = 0;
-  return 0;
-}
+//       *it = b->next;
+//       unsigned int res = b->val;
+//       free_string(b->key);
+//       free_blist(b);
+//       *removed = 1;
+//       return res;
+//     }
+//   }
+//   *removed = 0;
+//   return 0;
+// }
 
-void hashtbl_free_blist(struct blist *bl)
-/*@
-  With l ls m1 m2 lh b h lhx k key v
-  Require map_composable(m1, m2) &&
-          contain_all_addrs(m1, l) && 
-          repr_all_heads(lh, b) && 
-          contain_all_correct_addrs(m1, b) && 
-          dll(h->top, (void*) 0, l) * 
-          sll(lhx, ls) *
-          store_map(store_name, m1) *
-          store_map(store_uint, m2) *
-          (bl == (void*) 0 ||
-          (bl != (void *) 0 &&
-          store_ptr(&(bl->key), key) *
-          store_string(key, k) *
-          store_uint(&(bl->val), v)))
-  Ensure exists l0 l_up l_down l1 ls0 ls1 k,
-          map_composable(m1, m2) &&
-          contain_all_addrs(m1, l1) && 
-          repr_all_heads(lh, b) && 
-          contain_all_correct_addrs(m1, b) && 
-          ((bl != (void *) 0 &&
-          l0 == app(l_up, l_down) &&
-          l1 == cons(bl, l_down) &&
-          l == app(l_up, l1) &&
-          ls1 == cons(bl, nil) &&
-          ls == app(ls0, ls1) &&
-          sll(lhx, ls0) *
-          dll(h->top, (void*) 0, l0) * 
-          store_map(store_name, KP::remove_map(m1, k)) *
-          store_map(store_uint, PV::remove_map(m2, bl))) ||
-          (bl == (void *) 0 && 
-          dll(h->top, (void*) 0, l) * 
-          sll(lhx, ls) *
-          store_map(store_name, m1) *
-          store_map(store_uint, m2)))
-*/
-{
-  if (bl != (void *) 0) {
-    /*@ bl != 0 
-        which implies
-        exists key k v,
-        store_ptr(&(bl->key), key) *
-        store_string(key, k) *
-        store_uint(&(bl->val), v)
-    */
-    hashtbl_free_blist(bl->next);
-    free_string(bl -> key);
-    free_blist(bl);
-  }
-}
+// void hashtbl_free_blist(struct blist *bl)
+// /*@
+//   With l ls m1 m2 lh b h lhx k key v
+//   Require map_composable(m1, m2) &&
+//           contain_all_addrs(m1, l) && 
+//           repr_all_heads(lh, b) && 
+//           contain_all_correct_addrs(m1, b) && 
+//           dll(h->top, (void*) 0, l) * 
+//           sll(lhx, ls) *
+//           store_map(store_name, m1) *
+//           store_map(store_uint, m2) *
+//           (bl == (void*) 0 ||
+//           (bl != (void *) 0 &&
+//           store_ptr(&(bl->key), key) *
+//           store_string(key, k) *
+//           store_uint(&(bl->val), v)))
+//   Ensure exists l0 l_up l_down l1 ls0 ls1 k,
+//           map_composable(m1, m2) &&
+//           contain_all_addrs(m1, l1) && 
+//           repr_all_heads(lh, b) && 
+//           contain_all_correct_addrs(m1, b) && 
+//           ((bl != (void *) 0 &&
+//           l0 == app(l_up, l_down) &&
+//           l1 == cons(bl, l_down) &&
+//           l == app(l_up, l1) &&
+//           ls1 == cons(bl, nil) &&
+//           ls == app(ls0, ls1) &&
+//           sll(lhx, ls0) *
+//           dll(h->top, (void*) 0, l0) * 
+//           store_map(store_name, KP::remove_map(m1, k)) *
+//           store_map(store_uint, PV::remove_map(m2, bl))) ||
+//           (bl == (void *) 0 && 
+//           dll(h->top, (void*) 0, l) * 
+//           sll(lhx, ls) *
+//           store_map(store_name, m1) *
+//           store_map(store_uint, m2)))
+// */
+// {
+//   if (bl != (void *) 0) {
+//     /*@ bl != 0 
+//         which implies
+//         exists key k v,
+//         store_ptr(&(bl->key), key) *
+//         store_string(key, k) *
+//         store_uint(&(bl->val), v)
+//     */
+//     hashtbl_free_blist(bl->next);
+//     free_string(bl -> key);
+//     free_blist(bl);
+//   }
+// }
 
-void hashtbl_clear(struct hashtbl *h)
-/*@
-  With m1 m2
-  Require map_composable(m1, m2) &&
-          store_hash_skeleton(h, m1) *
-          store_map(store_uint, m2)
-  Ensure has_ptr_permission(&(h->bucks)) * 
-         has_ptr_permission(&(h->top)) *
-         store_map(store_name, m1) * 
-         store_map(store_uint, m2)
-*/ 
-{
-  /*@ store_hash_skeleton(h, m1)
-      which implies
-        exists l lh b, 
-        contain_all_addrs(m1, l) && 
-        repr_all_heads(lh, b) && 
-        contain_all_correct_addrs(m1, b) && 
-        dll(h->top, (void*) 0, l) * 
-        IntArray::full(h->bucks, 211, lh) * 
-        store_map(store_sll, b)*
-        store_map(store_name, m1)
-  */
-  int i;
-  /*@ Inv Assert
-      exists li k buck lh,
-      map_composable(m1, m2) &&
-      sll(buck, li) *
-      store_map(store_name, m1) *
-      store_map(store_uint, m2) *
-      store_string(buck->key, k) *
-      store(&h->bucks[i], buck) *
-      IntArray::full(h->bucks, 211, lh) *
-      has_ptr_permission(h->top)
-  */
-  for (i = 0; i < 211; i++) {
-    hashtbl_free_blist(h->bucks[i]);
-    h->bucks[i] = (void *) 0;
-  }
+// void hashtbl_clear(struct hashtbl *h)
+// /*@
+//   With m1 m2
+//   Require map_composable(m1, m2) &&
+//           store_hash_skeleton(h, m1) *
+//           store_map(store_uint, m2)
+//   Ensure has_ptr_permission(&(h->bucks)) * 
+//          has_ptr_permission(&(h->top)) *
+//          store_map(store_name, m1) * 
+//          store_map(store_uint, m2)
+// */ 
+// {
+//   /*@ store_hash_skeleton(h, m1)
+//       which implies
+//         exists l lh b, 
+//         contain_all_addrs(m1, l) && 
+//         repr_all_heads(lh, b) && 
+//         contain_all_correct_addrs(m1, b) && 
+//         dll(h->top, (void*) 0, l) * 
+//         IntArray::full(h->bucks, 211, lh) * 
+//         store_map(store_sll, b)*
+//         store_map(store_name, m1)
+//   */
+//   int i;
+//   /*@ Inv Assert
+//       exists li k buck lh,
+//       map_composable(m1, m2) &&
+//       sll(buck, li) *
+//       store_map(store_name, m1) *
+//       store_map(store_uint, m2) *
+//       store_string(buck->key, k) *
+//       store(&h->bucks[i], buck) *
+//       IntArray::full(h->bucks, 211, lh) *
+//       has_ptr_permission(h->top)
+//   */
+//   for (i = 0; i < 211; i++) {
+//     hashtbl_free_blist(h->bucks[i]);
+//     h->bucks[i] = (void *) 0;
+//   }
 
-  free_blist_array(h->bucks);
-  h->bucks = (void *) 0;
-  h->top = (void *) 0;
-}
+//   free_blist_array(h->bucks);
+//   h->bucks = (void *) 0;
+//   h->top = (void *) 0;
+// }
 
-void free_hashtbl(struct hashtbl *h)
-/*@
-  With m1 m2
-  Require map_composable(m1, m2) &&
-          store_hash_skeleton(h, m1) *
-          store_map(store_uint, m2)
-  Ensure emp
-*/
-{
-  hashtbl_clear(h);
-  free_hashtbl_struct(h);
-}
+// void free_hashtbl(struct hashtbl *h)
+// /*@
+//   With m1 m2
+//   Require map_composable(m1, m2) &&
+//           store_hash_skeleton(h, m1) *
+//           store_map(store_uint, m2)
+//   Ensure emp
+// */
+// {
+//   hashtbl_clear(h);
+//   free_hashtbl_struct(h);
+// }
