HashTable/hashtbl_proof_auto.v
@@ -39,6 +39,12 @@ Proof. Admitted.
 Lemma proof_of_hashtbl_findref_safety_wit_6 : hashtbl_findref_safety_wit_6.
 Proof. Admitted. 
 
+Lemma proof_of_hashtbl_findref_safety_wit_7 : hashtbl_findref_safety_wit_7.
+Proof. Admitted. 
+
+Lemma proof_of_hashtbl_findref_safety_wit_8 : hashtbl_findref_safety_wit_8.
+Proof. Admitted. 
+
 Lemma proof_of_hashtbl_findref_entail_wit_2_1 : hashtbl_findref_entail_wit_2_1.
 Proof. Admitted. 
 
