HashTable/hashtbl_proof_manual.v
@@ -21,76 +21,28 @@ Require Import hashtbl_lib.
 Require Import hashtbl_lib.
 Local Open Scope sac.
 
+Lemma proof_of_hashtbl_findref_safety_wit_9 : hashtbl_findref_safety_wit_9.
+Proof. 
+    pre_process.
+Qed.
+
 Lemma proof_of_hashtbl_findref_entail_wit_1 : hashtbl_findref_entail_wit_1.
 Proof. 
     pre_process.
-    unfold contain_all_addrs in *.
-    unfold repr_all_heads in *.
-    unfold contain_all_correct_addrs in *.
-    prop_apply (IntArray.full_Zlength h_bucks 211 lh_2).
-    entailer!.
-    repeat rewrite derivable1_sepcon_assoc1 in *.
-    assert (0 <= retval % 211 < 211) as Hrem.
-    {entailer!. 
-        + apply Z.rem_nonneg; [lia | ].
-            subst retval.
-            apply hash_string_in_range.
-        + apply Z.rem_bound_pos; [ |lia].
-            subst retval.
-            apply hash_string_in_range.
-            }
-    assert (exists p, Znth (retval % 211) lh_2 0 = p) as [p Hp].
-    { exists (Znth (retval % 211) lh_2 0); reflexivity. }
-    assert (exists l, b0_2 (retval % 211) = Some (p, l)) as [l0 Hb0].
-    { apply H1. split; auto.
-      split.
-      entailer!.
-      rewrite <-H3.
-      apply Z.rem_bound_pos.
-      + subst retval.
-        apply hash_string_in_range.
-      + unfold Zlength in H3.
-        unfold Zlength.
-        assert (Zlength_aux 0 addr lh_2 = Zlength_aux 0 Z lh_2).
-        {
-            reflexivity.
-        }
-        rewrite H4.
-        rewrite H3.
-        lia.
-     }
-    Exists h_bucks key_pre h_top_2 p k.
-    Exists l0 h_bucks l0 nil.
-    Exists lh_2 b0_2 l_2.
-    entailer!.
-    3: {
-
-    }
-    unfold IntArray.full.
-    Search store_array.
-    rewrite (store_array_split_to_missing_i Z (fun (x : addr) (lo a : Z) =>
-                                                (x + lo * sizeof ( INT )) # Int |-> a)
-                                                h_bucks (retval%211) 211 lh_2 (h_bucks + retval % 211 * sizeof ( PTR ))).
-    
-    Search sepcon.
-    (* repeat rewrite derivable1_sepcon_assoc1. *)
-    entailer!.
+    rewrite <- derivable1_orp_intros1.
+    Exists h_top_3 h_bucks 0 buck.
 Admitted. 
 
 Lemma proof_of_hashtbl_findref_entail_wit_4 : hashtbl_findref_entail_wit_4.
-Proof.
-    pre_process.
-    destruct l_res_2.
-    + Exists buck k0 h_top i_v_2 k_list_2.
-        Exists l_res_2 h_bucks_2 l0_2.
-        Exists l_prev_2 lh_2 b0_2 l.
-
- Admitted. 
+Proof. Admitted. 
 
 Lemma proof_of_hashtbl_findref_return_wit_1 : hashtbl_findref_return_wit_1.
 Proof. Admitted. 
 
 Lemma proof_of_hashtbl_findref_return_wit_2 : hashtbl_findref_return_wit_2.
+Proof. Admitted. 
+
+Lemma proof_of_hashtbl_findref_return_wit_3 : hashtbl_findref_return_wit_3.
 Proof. Admitted. 
 
 Lemma proof_of_hashtbl_findref_which_implies_wit_1 : hashtbl_findref_which_implies_wit_1.
